verified/kev_common.dfy
@@ -1,0 +1,148 @@
+include "ARMspartan.dfy"
+include "kev_constants.dfy"
+include "pagedb.dfy"
+
+//-----------------------------------------------------------------------------
+// Globals
+//-----------------------------------------------------------------------------
+
+function method {:opaque} PageDb(): operand { op_sym("g_pagedb") }
+function method {:opaque} SecurePhysBaseOp(): operand { op_sym("g_secure_physbase") }
+
+// the phys base is unknown, but never changes
+function {:axiom} SecurePhysBase(): int
+    ensures 0 < SecurePhysBase() <= KEVLAR_PHYSMEM_LIMIT() - KEVLAR_SECURE_RESERVE();
+    ensures WordAligned(SecurePhysBase());
+
+function method KevGlobalDecls(): globaldecls
+    ensures ValidGlobalDecls(KevGlobalDecls());
+{
+    reveal_PageDb(); reveal_SecurePhysBaseOp();
+    GlobalDecls(map[SecurePhysBaseOp() := 4, //BytesPerWord()
+                    PageDb() := G_PAGEDB_SIZE()])
+}
+
+
+//-----------------------------------------------------------------------------
+// Stack
+//-----------------------------------------------------------------------------
+
+// we don't know where the stack is exactly, but we know how big it is
+function {:axiom} StackLimit():int
+    ensures WordAligned(StackLimit())
+    ensures KEVLAR_MON_VBASE() <= StackLimit()
+    ensures StackLimit() <= KEVLAR_DIRECTMAP_VBASE() - KEVLAR_STACK_SIZE()
+
+function StackBase():int
+{
+    StackLimit() + KEVLAR_STACK_SIZE()
+}
+
+predicate ValidStack(s:state)
+    requires ValidState(s)
+{
+    WordAligned(eval_op(s, op_sp()))
+    && StackLimit() < eval_op(s, op_sp()) <= StackBase()
+}
+
+predicate StackBytesRemaining(s:state,bytes:int)
+{
+    ValidState(s) && ValidStack(s) &&
+    (StackLimit() + bytes < eval_op(s,op_sp()) <= StackBase())
+}
+
+predicate ParentStackPreserving(s:state, r:state)
+    requires SaneState(s) && SaneState(r)
+{
+    var sp := eval_op(s,op_sp());
+    forall i :: sp <= i < StackBase() && WordAligned(i) ==> addrval(r,i) == addrval(s,i)
+}
+
+predicate StackPreserving(s:state, r:state)
+    requires SaneState(s) && SaneState(r)
+{
+    eval_op(s,op_sp()) == eval_op(r,op_sp())
+    && ParentStackPreserving(s, r)
+}
+
+
+//-----------------------------------------------------------------------------
+// Procedure invariants
+//-----------------------------------------------------------------------------
+
+predicate RegPreservingExcept(s:state, r:state, trashed:seq<operand>)
+    requires ValidState(s) && ValidState(r);
+    requires forall o :: o in trashed ==> ValidRegOperand(o);
+{
+    forall reg {:trigger OReg(reg)} :: OReg(reg) !in trashed && ValidRegOperand(OReg(reg))
+        ==> eval_op(s,OReg(reg)) == eval_op(r,OReg(reg))
+    && (op_sp() !in trashed ==> eval_op(s,op_sp()) == eval_op(r,op_sp()))
+    && (op_lr() !in trashed ==> eval_op(s,op_lr()) == eval_op(r,op_lr()))
+}
+
+predicate NonvolatileRegPreserving(s:state, r:state)
+    requires ValidState(s) && ValidState(r);
+{
+    RegPreservingExcept(s, r, [OReg(R0), OReg(R1), OReg(R2), OReg(R3)])
+}
+
+predicate MemPreservingExcept(s:state, r:state, base:int, limit:int)
+    requires AlwaysInvariant(s,r);
+    requires limit >= base;
+{
+    forall i :: ValidMem(s.m,i) && (i < base || i >= limit) ==> addrval(s,i) == addrval(r,i)
+}
+
+predicate NonStackMemPreserving(s:state, r:state)
+    requires AlwaysInvariant(s,r);
+{
+    MemPreservingExcept(s, r, StackLimit(), StackBase())
+}
+
+
+//-----------------------------------------------------------------------------
+// Application-level state invariants
+//-----------------------------------------------------------------------------
+
+predicate SaneMem(s:memstate)
+{
+    ValidMemState(s)
+    // TODO: our insecure phys mapping must be valid
+    //&& ValidMemRange(s, KEVLAR_DIRECTMAP_VBASE(),
+    //    (KEVLAR_DIRECTMAP_VBASE() + MonitorPhysBaseValue()))
+    // our secure phys mapping must be valid
+    && ValidMemRange(s, KEVLAR_DIRECTMAP_VBASE() + SecurePhysBase(),
+        (KEVLAR_DIRECTMAP_VBASE() + SecurePhysBase() + KEVLAR_SECURE_RESERVE()))
+    // the stack must be mapped
+    && ValidMemRange(s, StackLimit(), StackBase())
+    // globals are as we expect
+    && KevGlobalDecls() == TheGlobalDecls()
+    && GlobalFullContents(s, SecurePhysBaseOp()) == [SecurePhysBase()]
+    // XXX: workaround so dafny sees that these are distinct
+    && SecurePhysBaseOp() != PageDb()
+}
+
+predicate SaneState(s:state)
+{
+    ValidState(s) && ValidStack(s) && SaneMem(s.m) && mode_of_state(s) == Monitor
+}
+
+
+//-----------------------------------------------------------------------------
+// Common functions
+//-----------------------------------------------------------------------------
+
+function page_paddr(p: PageNr) : int
+    requires validPageNr(p)
+    ensures WordAligned(page_paddr(p))
+{
+    assert WordAligned(KEVLAR_PAGE_SIZE());
+    SecurePhysBase() + p * KEVLAR_PAGE_SIZE()
+}
+
+function page_monvaddr(pagenr:PageNr):int
+    requires validPageNr(pagenr)
+    ensures WordAligned(page_monvaddr(pagenr))
+{
+    page_paddr(pagenr) + KEVLAR_DIRECTMAP_VBASE()
+}
