verified/pagedb_impl.dfy
@@ -1,0 +1,136 @@
+include "pagedb.dfy"
+include "kev_common.dfy"
+
+predicate addrInPage(m:mem, p:PageNr)
+    requires validPageNr(p)
+{
+    WordAligned(m) && page_monvaddr(p) <= m < page_monvaddr(p) + KEVLAR_PAGE_SIZE()
+}
+
+predicate memContainsPage(memmap: map<mem, int>, p:PageNr)
+    requires validPageNr(p)
+{
+    forall m :: addrInPage(m,p) ==> m in memmap
+}
+
+function extractPage(s:memstate, p:PageNr): map<mem, int>
+    requires SaneMem(s)
+    requires validPageNr(p)
+    ensures memContainsPage(extractPage(s,p), p)
+{
+    // XXX: expanded addrInPage() to help Dafny see a bounded set
+    (map m | WordAligned(m)
+        && page_monvaddr(p) <= m < page_monvaddr(p) + KEVLAR_PAGE_SIZE()
+        :: s.addresses[m])
+}
+
+function extractPageDbEntry(s:memstate, p:PageNr): seq<int>
+    requires SaneMem(s)
+    requires validPageNr(p)
+    ensures |extractPageDbEntry(s,p)| == BytesToWords(PAGEDB_ENTRY_SIZE())
+    ensures forall o :: WordAligned(o) && 0 <= o < PAGEDB_ENTRY_SIZE()
+        ==> GlobalWord(s, PageDb(), G_PAGEDB_ENTRY(p) + o)
+            == extractPageDbEntry(s,p)[BytesToWords(o)]
+{
+    var fulldb := GlobalFullContents(s, PageDb());
+    assert |fulldb| == BytesToWords(G_PAGEDB_SIZE());
+    var entrylen := BytesToWords(PAGEDB_ENTRY_SIZE());
+    fulldb[p*entrylen..p*entrylen+entrylen]
+}
+
+predicate pageDbCorresponds(s:memstate, pagedb:PageDb)
+    requires SaneMem(s)
+    requires pageDbClosedRefs(pagedb)
+{
+    // XXX: unpack the entry and page contents here to help dafny see
+    // that we have no other dependencies on the state
+    var db := (map p | 0 <= p < KEVLAR_SECURE_NPAGES() :: extractPageDbEntry(s,p));
+    var secpages := (map p | 0 <= p < KEVLAR_SECURE_NPAGES() :: extractPage(s,p));
+    forall p {:trigger validPageNr(p)} :: validPageNr(p)
+        ==> (pageDbEntryCorresponds(p, pagedb[p], db[p])
+            && pageContentsCorresponds(p, pagedb[p], secpages[p]))
+}
+
+predicate pageDbCorrespondsExcluding(s:memstate, pagedb:PageDb, modifiedPage:PageNr)
+    requires SaneMem(s)
+    requires pageDbClosedRefs(pagedb)
+{
+    forall p {:trigger validPageNr(p)} :: validPageNr(p) && p != modifiedPage
+        ==> (pageDbEntryCorresponds(p, pagedb[p], extractPageDbEntry(s, p))
+            && pageContentsCorresponds(p, pagedb[p], extractPage(s, p)))
+}
+
+predicate pageDbCorrespondsOnly(s:memstate, pagedb:PageDb, p:PageNr)
+    requires SaneMem(s)
+    requires pageDbClosedRefs(pagedb)
+    requires validPageNr(p)
+{
+    pageDbEntryCorresponds(p, pagedb[p], extractPageDbEntry(s, p))
+    && pageContentsCorresponds(p, pagedb[p], extractPage(s, p))
+}
+
+predicate {:opaque} pageDbEntryCorresponds(p:PageNr, e:PageDbEntry, entryWords:seq<int>)
+    requires validPageNr(p)
+    requires |entryWords| == BytesToWords(PAGEDB_ENTRY_SIZE())
+    requires e.PageDbEntryTyped?
+        ==> validPageNr(e.addrspace) && closedRefsPageDbEntry(e.entry)
+{
+    pageDbEntryTypeVal(e) == entryWords[BytesToWords(PAGEDB_ENTRY_TYPE())]
+    && match e {
+        case PageDbEntryFree => true
+        case PageDbEntryTyped(addrspace, entry) =>
+            entryWords[BytesToWords(PAGEDB_ENTRY_ADDRSPACE())]
+                == page_monvaddr(addrspace)
+    }
+}
+
+predicate {:opaque} pageContentsCorresponds(p:PageNr, e:PageDbEntry, page:map<mem, int>)
+    requires validPageNr(p)
+    requires memContainsPage(page, p)
+    requires e.PageDbEntryFree? || closedRefsPageDbEntry(e.entry)
+{
+    e.PageDbEntryFree? || (e.PageDbEntryTyped? && (
+        var et := e.entry;
+        (et.Addrspace? && pageDbAddrspaceCorresponds(p, et, page))
+        || (et.Dispatcher? /* && pageDbDispatcherCorresponds(p, et, page) */)
+        || (et.L1PTable? /* && pageDbL1PTableCorresponds(p, et, page) */)
+        || (et.L2PTable? /* && pageDbL2PTableCorresponds(p, et, page) */)
+        || et.DataPage?))
+}
+
+predicate pageDbAddrspaceCorresponds(p:PageNr, e:PageDbEntryTyped, page:map<mem, int>)
+    requires validPageNr(p)
+    requires memContainsPage(page, p)
+    requires e.Addrspace?
+    requires closedRefsPageDbEntry(e)
+{
+    var base := page_monvaddr(p);
+    assert base in page;
+    page[ADDRSPACE_L1PT(base)] == page_monvaddr(e.l1ptnr)
+    && page[ADDRSPACE_L1PT_PHYS(base)] == page_paddr(e.l1ptnr)
+    && page[ADDRSPACE_REF(base)] == e.refcount
+    && page[ADDRSPACE_STATE(base)] == pageDbAddrspaceStateVal(e.state)
+}
+
+function pageDbEntryTypeVal(e: PageDbEntry): int
+    ensures isUInt32(pageDbEntryTypeVal(e))
+{
+    if e.PageDbEntryFree? then KEV_PAGE_FREE()
+    else match e.entry {
+    case Addrspace(l1pt, ref, state) => KEV_PAGE_ADDRSPACE()
+    case Dispatcher(ep, entered) => KEV_PAGE_DISPATCHER()
+    case L1PTable(pt) => KEV_PAGE_L1PTABLE()
+    case L2PTable(pt) => KEV_PAGE_L2PTABLE()
+    case DataPage => KEV_PAGE_DATA()
+    }
+}
+
+function pageDbAddrspaceStateVal(s: AddrspaceState): int
+    ensures isUInt32(pageDbAddrspaceStateVal(s))
+{
+    match s {
+    case InitState => KEV_ADDRSPACE_INIT()
+    case FinalState => KEV_ADDRSPACE_FINAL()
+    case StoppedState => KEV_ADDRSPACE_STOPPED()
+    }
+}
